{-# OPTIONS --without-K #-}

module Pif2 where

{-- 2 paths --} 

open import Level using (Level; _⊔_) renaming (zero to lzero; suc to lsuc)

open import Relation.Binary.PropositionalEquality 
  using (_≡_; refl; sym; trans; subst; subst₂; cong; cong₂; setoid; 
        proof-irrelevance; module ≡-Reasoning)
open import Relation.Binary.PropositionalEquality.TrustMe
  using (trustMe)
open import Relation.Nullary.Core using (Dec; yes; no; ¬_)
open import Data.Nat.Properties using (m≢1+m+n; i+j≡0⇒i≡0; i+j≡0⇒j≡0)
open import Data.Nat.Properties.Simple 
  using (+-right-identity; +-suc; +-assoc; +-comm; 
        *-assoc; *-comm; *-right-zero; distribʳ-*-+)
open import Data.Nat.DivMod using (_mod_)
open import Relation.Binary using (Rel; Decidable; Setoid)
open import Relation.Binary.Core using (Transitive)

open import Data.String using (String)
  renaming (_++_ to _++S_)
open import Data.Nat.Show using (show)
open import Data.Bool using (Bool; false; true)
open import Data.Nat using (ℕ; suc; _+_; _∸_; _*_; _<_; _≮_; _≤_; _≰_; 
  z≤n; s≤s; _≟_; _≤?_; module ≤-Reasoning)
open import Data.Fin 
  using (Fin; zero; suc; toℕ; fromℕ; _ℕ-_; _≺_;
         raise; inject+; inject₁; inject≤; _≻toℕ_) 
  renaming (_+_ to _F+_)
open import Data.Fin.Properties using (bounded; inject+-lemma)
open import Data.Vec.Properties 
  using (lookup∘tabulate; tabulate∘lookup; lookup-allFin; tabulate-∘; 
         tabulate-allFin; map-id; allFin-map)

open import Data.List 
  using (List; []; _∷_; _∷ʳ_; foldl; replicate; reverse; downFrom; 
         concatMap; gfilter; initLast; InitLast; _∷ʳ'_) 
  renaming (_++_ to _++L_; map to mapL; concat to concatL; zip to zipL)
open import Data.List.NonEmpty 
  using (List⁺; [_]; _∷⁺_; head; last; _⁺++_)
  renaming (toList to nonEmptyListtoList; _∷ʳ_ to _n∷ʳ_; tail to ntail)
open import Data.List.Any using (Any; here; there; any; module Membership)
open import Data.Maybe using (Maybe; nothing; just; maybe′)
open import Data.Vec 
  using (Vec; tabulate; []; _∷_; tail; lookup; zip; zipWith; splitAt;
         _[_]≔_; allFin; toList)
  renaming (_++_ to _++V_; map to mapV; concat to concatV)
open import Function using (id; _∘_; _$_)

open import Data.Empty   using (⊥; ⊥-elim)
open import Data.Unit    using (⊤; tt)
open import Data.Sum     using (_⊎_; inj₁; inj₂)
open import Data.Product using (_×_; _,_; proj₁; proj₂)

open import Cauchy
open import Perm
open import Proofs
open import CauchyProofs
open import CauchyProofsT
open import CauchyProofsS
open import Groupoid
open import Pif

------------------------------------------------------------------------------
-- Picture so far:
--
--           path p
--   =====================
--  ||   ||             ||
--  ||   ||2path        ||
--  ||   ||             ||
--  ||   ||  path q     ||
--  t₁ =================t₂
--  ||   ...            ||
--   =====================
--
-- The types t₁, t₂, etc are discrete groupoids. The paths between
-- them correspond to permutations. Each syntactically different
-- permutation corresponds to a path but equivalent permutations are
-- connected by 2paths.  But now we want an alternative definition of
-- 2paths that is structural, i.e., that looks at the actual
-- construction of the path t₁ ⟷ t₂ in terms of combinators... The
-- theorem we want is that α ∼ β iff we can rewrite α to β using
-- various syntactic structural rules. We start with a collection of
-- simplication rules and then try to show they are complete.

-- Simplification rules

infix  30 _⇔_

data _⇔_ : {t₁ t₂ : U} → (t₁ ⟷ t₂) → (t₁ ⟷ t₂) → Set where
  assoc◎l : {t₁ t₂ t₃ t₄ : U} {c₁ : t₁ ⟷ t₂} {c₂ : t₂ ⟷ t₃} {c₃ : t₃ ⟷ t₄} → 
          (c₁ ◎ (c₂ ◎ c₃)) ⇔ ((c₁ ◎ c₂) ◎ c₃)
  assoc◎r : {t₁ t₂ t₃ t₄ : U} {c₁ : t₁ ⟷ t₂} {c₂ : t₂ ⟷ t₃} {c₃ : t₃ ⟷ t₄} → 
          ((c₁ ◎ c₂) ◎ c₃) ⇔ (c₁ ◎ (c₂ ◎ c₃))
  assoc⊕l : {t₁ t₂ t₃ t₄ t₅ t₆ : U} 
          {c₁ : t₁ ⟷ t₂} {c₂ : t₃ ⟷ t₄} {c₃ : t₅ ⟷ t₆} → 
          (c₁ ⊕ (c₂ ⊕ c₃)) ⇔ (assocl₊ ◎ ((c₁ ⊕ c₂) ⊕ c₃) ◎ assocr₊)
  assoc⊕r : {t₁ t₂ t₃ t₄ t₅ t₆ : U} 
          {c₁ : t₁ ⟷ t₂} {c₂ : t₃ ⟷ t₄} {c₃ : t₅ ⟷ t₆} → 
          (assocl₊ ◎ ((c₁ ⊕ c₂) ⊕ c₃) ◎ assocr₊) ⇔ (c₁ ⊕ (c₂ ⊕ c₃))
  assoc⊗l : {t₁ t₂ t₃ t₄ t₅ t₆ : U} 
          {c₁ : t₁ ⟷ t₂} {c₂ : t₃ ⟷ t₄} {c₃ : t₅ ⟷ t₆} → 
          (c₁ ⊗ (c₂ ⊗ c₃)) ⇔ (assocl⋆ ◎ ((c₁ ⊗ c₂) ⊗ c₃) ◎ assocr⋆)
  assoc⊗r : {t₁ t₂ t₃ t₄ t₅ t₆ : U} 
          {c₁ : t₁ ⟷ t₂} {c₂ : t₃ ⟷ t₄} {c₃ : t₅ ⟷ t₆} → 
          (assocl⋆ ◎ ((c₁ ⊗ c₂) ⊗ c₃) ◎ assocr⋆) ⇔ (c₁ ⊗ (c₂ ⊗ c₃))
  dist⇔ : {t₁ t₂ t₃ t₄ t₅ t₆ : U} 
          {c₁ : t₁ ⟷ t₂} {c₂ : t₃ ⟷ t₄} {c₃ : t₅ ⟷ t₆} → 
          ((c₁ ⊕ c₂) ⊗ c₃) ⇔ (dist ◎ ((c₁ ⊗ c₃) ⊕ (c₂ ⊗ c₃)) ◎ factor)
  factor⇔ : {t₁ t₂ t₃ t₄ t₅ t₆ : U} 
          {c₁ : t₁ ⟷ t₂} {c₂ : t₃ ⟷ t₄} {c₃ : t₅ ⟷ t₆} → 
          (dist ◎ ((c₁ ⊗ c₃) ⊕ (c₂ ⊗ c₃)) ◎ factor) ⇔ ((c₁ ⊕ c₂) ⊗ c₃)
  idl◎l   : {t₁ t₂ : U} {c : t₁ ⟷ t₂} → (id⟷ ◎ c) ⇔ c
  idl◎r   : {t₁ t₂ : U} {c : t₁ ⟷ t₂} → c ⇔ id⟷ ◎ c
  idr◎l   : {t₁ t₂ : U} {c : t₁ ⟷ t₂} → (c ◎ id⟷) ⇔ c
  idr◎r   : {t₁ t₂ : U} {c : t₁ ⟷ t₂} → c ⇔ (c ◎ id⟷) 
  linv◎l  : {t₁ t₂ : U} {c : t₁ ⟷ t₂} → (c ◎ ! c) ⇔ id⟷
  linv◎r  : {t₁ t₂ : U} {c : t₁ ⟷ t₂} → id⟷ ⇔ (c ◎ ! c) 
  rinv◎l  : {t₁ t₂ : U} {c : t₁ ⟷ t₂} → (! c ◎ c) ⇔ id⟷
  rinv◎r  : {t₁ t₂ : U} {c : t₁ ⟷ t₂} → id⟷ ⇔ (! c ◎ c) 
  unitel₊⇔ : {t₁ t₂ : U} {c₁ : ZERO ⟷ ZERO} {c₂ : t₁ ⟷ t₂} → 
          (unite₊ ◎ c₂) ⇔ ((c₁ ⊕ c₂) ◎ unite₊)
  uniter₊⇔ : {t₁ t₂ : U} {c₁ : ZERO ⟷ ZERO} {c₂ : t₁ ⟷ t₂} → 
          ((c₁ ⊕ c₂) ◎ unite₊) ⇔ (unite₊ ◎ c₂)
  unitil₊⇔ : {t₁ t₂ : U} {c₁ : ZERO ⟷ ZERO} {c₂ : t₁ ⟷ t₂} → 
          (uniti₊ ◎ (c₁ ⊕ c₂)) ⇔ (c₂ ◎ uniti₊)
  unitir₊⇔ : {t₁ t₂ : U} {c₁ : ZERO ⟷ ZERO} {c₂ : t₁ ⟷ t₂} → 
          (c₂ ◎ uniti₊) ⇔ (uniti₊ ◎ (c₁ ⊕ c₂))
  unitial₊⇔ : {t₁ t₂ : U} → (uniti₊ {PLUS t₁ t₂} ◎ assocl₊) ⇔ (uniti₊ ⊕ id⟷)
  unitiar₊⇔ : {t₁ t₂ : U} → (uniti₊ {t₁} ⊕ id⟷ {t₂}) ⇔ (uniti₊ ◎ assocl₊)
  swapl₊⇔ : {t₁ t₂ t₃ t₄ : U} {c₁ : t₁ ⟷ t₂} {c₂ : t₃ ⟷ t₄} → 
          (swap₊ ◎ (c₁ ⊕ c₂)) ⇔ ((c₂ ⊕ c₁) ◎ swap₊)
  swapr₊⇔ : {t₁ t₂ t₃ t₄ : U} {c₁ : t₁ ⟷ t₂} {c₂ : t₃ ⟷ t₄} → 
          ((c₂ ⊕ c₁) ◎ swap₊) ⇔ (swap₊ ◎ (c₁ ⊕ c₂))
  unitel⋆⇔ : {t₁ t₂ : U} {c₁ : ONE ⟷ ONE} {c₂ : t₁ ⟷ t₂} → 
          (unite⋆ ◎ c₂) ⇔ ((c₁ ⊗ c₂) ◎ unite⋆)
  uniter⋆⇔ : {t₁ t₂ : U} {c₁ : ONE ⟷ ONE} {c₂ : t₁ ⟷ t₂} → 
          ((c₁ ⊗ c₂) ◎ unite⋆) ⇔ (unite⋆ ◎ c₂)
  unitil⋆⇔ : {t₁ t₂ : U} {c₁ : ONE ⟷ ONE} {c₂ : t₁ ⟷ t₂} → 
          (uniti⋆ ◎ (c₁ ⊗ c₂)) ⇔ (c₂ ◎ uniti⋆)
  unitir⋆⇔ : {t₁ t₂ : U} {c₁ : ONE ⟷ ONE} {c₂ : t₁ ⟷ t₂} → 
          (c₂ ◎ uniti⋆) ⇔ (uniti⋆ ◎ (c₁ ⊗ c₂))
  unitial⋆⇔ : {t₁ t₂ : U} → (uniti⋆ {TIMES t₁ t₂} ◎ assocl⋆) ⇔ (uniti⋆ ⊗ id⟷)
  unitiar⋆⇔ : {t₁ t₂ : U} → (uniti⋆ {t₁} ⊗ id⟷ {t₂}) ⇔ (uniti⋆ ◎ assocl⋆)
  swapl⋆⇔ : {t₁ t₂ t₃ t₄ : U} {c₁ : t₁ ⟷ t₂} {c₂ : t₃ ⟷ t₄} → 
          (swap⋆ ◎ (c₁ ⊗ c₂)) ⇔ ((c₂ ⊗ c₁) ◎ swap⋆)
  swapr⋆⇔ : {t₁ t₂ t₃ t₄ : U} {c₁ : t₁ ⟷ t₂} {c₂ : t₃ ⟷ t₄} → 
          ((c₂ ⊗ c₁) ◎ swap⋆) ⇔ (swap⋆ ◎ (c₁ ⊗ c₂))
  swapfl⋆⇔ : {t₁ t₂ t₃ : U} → 
          (swap₊ {TIMES t₂ t₃} {TIMES t₁ t₃} ◎ factor) ⇔ 
          (factor ◎ (swap₊ {t₂} {t₁} ⊗ id⟷))
  swapfr⋆⇔ : {t₁ t₂ t₃ : U} → 
          (factor ◎ (swap₊ {t₂} {t₁} ⊗ id⟷)) ⇔ 
          (swap₊ {TIMES t₂ t₃} {TIMES t₁ t₃} ◎ factor)
  id⇔     : {t₁ t₂ : U} {c : t₁ ⟷ t₂} → c ⇔ c
  trans⇔  : {t₁ t₂ : U} {c₁ c₂ c₃ : t₁ ⟷ t₂} → 
          (c₁ ⇔ c₂) → (c₂ ⇔ c₃) → (c₁ ⇔ c₃)
  resp◎⇔  : {t₁ t₂ t₃ : U} 
          {c₁ : t₁ ⟷ t₂} {c₂ : t₂ ⟷ t₃} {c₃ : t₁ ⟷ t₂} {c₄ : t₂ ⟷ t₃} → 
          (c₁ ⇔ c₃) → (c₂ ⇔ c₄) → (c₁ ◎ c₂) ⇔ (c₃ ◎ c₄)
  resp⊕⇔  : {t₁ t₂ t₃ t₄ : U} 
          {c₁ : t₁ ⟷ t₂} {c₂ : t₃ ⟷ t₄} {c₃ : t₁ ⟷ t₂} {c₄ : t₃ ⟷ t₄} → 
          (c₁ ⇔ c₃) → (c₂ ⇔ c₄) → (c₁ ⊕ c₂) ⇔ (c₃ ⊕ c₄)
  resp⊗⇔  : {t₁ t₂ t₃ t₄ : U} 
          {c₁ : t₁ ⟷ t₂} {c₂ : t₃ ⟷ t₄} {c₃ : t₁ ⟷ t₂} {c₄ : t₃ ⟷ t₄} → 
          (c₁ ⇔ c₃) → (c₂ ⇔ c₄) → (c₁ ⊗ c₂) ⇔ (c₃ ⊗ c₄)

-- better syntax for writing 2paths

infix  2  _▤       
infixr 2  _⇔⟨_⟩_   

_⇔⟨_⟩_ : {t₁ t₂ : U} (c₁ : t₁ ⟷ t₂) {c₂ : t₁ ⟷ t₂} {c₃ : t₁ ⟷ t₂} → 
         (c₁ ⇔ c₂) → (c₂ ⇔ c₃) → (c₁ ⇔ c₃)
_ ⇔⟨ α ⟩ β = trans⇔ α β 

_▤ : {t₁ t₂ : U} → (c : t₁ ⟷ t₂) → (c ⇔ c)
_▤ c = id⇔ 

-- Inverses for 2paths

2! : {t₁ t₂ : U} {c₁ c₂ : t₁ ⟷ t₂} → (c₁ ⇔ c₂) → (c₂ ⇔ c₁)
2! assoc◎l = assoc◎r
2! assoc◎r = assoc◎l
2! assoc⊕l = assoc⊕r
2! assoc⊕r = assoc⊕l
2! assoc⊗l = assoc⊗r
2! assoc⊗r = assoc⊗l
2! dist⇔ = factor⇔ 
2! factor⇔ = dist⇔
2! idl◎l = idl◎r
2! idl◎r = idl◎l
2! idr◎l = idr◎r
2! idr◎r = idr◎l
2! linv◎l = linv◎r
2! linv◎r = linv◎l
2! rinv◎l = rinv◎r
2! rinv◎r = rinv◎l
2! unitel₊⇔ = uniter₊⇔
2! uniter₊⇔ = unitel₊⇔
2! unitil₊⇔ = unitir₊⇔
2! unitir₊⇔ = unitil₊⇔
2! swapl₊⇔ = swapr₊⇔
2! swapr₊⇔ = swapl₊⇔
2! unitial₊⇔ = unitiar₊⇔ 
2! unitiar₊⇔ = unitial₊⇔ 
2! unitel⋆⇔ = uniter⋆⇔
2! uniter⋆⇔ = unitel⋆⇔
2! unitil⋆⇔ = unitir⋆⇔
2! unitir⋆⇔ = unitil⋆⇔
2! unitial⋆⇔ = unitiar⋆⇔ 
2! unitiar⋆⇔ = unitial⋆⇔ 
2! swapl⋆⇔ = swapr⋆⇔
2! swapr⋆⇔ = swapl⋆⇔
2! swapfl⋆⇔ = swapfr⋆⇔
2! swapfr⋆⇔ = swapfl⋆⇔
2! id⇔ = id⇔
2! (trans⇔ α β) = trans⇔ (2! β) (2! α)
2! (resp◎⇔ α β) = resp◎⇔ (2! α) (2! β)
2! (resp⊕⇔ α β) = resp⊕⇔ (2! α) (2! β)
2! (resp⊗⇔ α β) = resp⊗⇔ (2! α) (2! β) 

-- a nice example of 2 paths

negEx : uniti⋆ ◎ (swap⋆ ◎ ((swap₊ {ONE} {ONE} ⊗ id⟷) ◎ (swap⋆ ◎ unite⋆))) 
        ⇔ swap₊
negEx = uniti⋆ ◎ (swap⋆ ◎ ((swap₊ ⊗ id⟷) ◎ (swap⋆ ◎ unite⋆)))
          ⇔⟨ resp◎⇔ id⇔ assoc◎l ⟩
        uniti⋆ ◎ ((swap⋆ ◎ (swap₊ ⊗ id⟷)) ◎ (swap⋆ ◎ unite⋆))
          ⇔⟨ resp◎⇔ id⇔ (resp◎⇔ swapl⋆⇔ id⇔) ⟩
        uniti⋆ ◎ (((id⟷ ⊗ swap₊) ◎ swap⋆) ◎ (swap⋆ ◎ unite⋆))
          ⇔⟨ resp◎⇔ id⇔ assoc◎r ⟩
        uniti⋆ ◎ ((id⟷ ⊗ swap₊) ◎ (swap⋆ ◎ (swap⋆ ◎ unite⋆)))
          ⇔⟨ resp◎⇔ id⇔ (resp◎⇔ id⇔ assoc◎l) ⟩
        uniti⋆ ◎ ((id⟷ ⊗ swap₊) ◎ ((swap⋆ ◎ swap⋆) ◎ unite⋆))
          ⇔⟨ resp◎⇔ id⇔ (resp◎⇔ id⇔ (resp◎⇔ linv◎l id⇔)) ⟩
        uniti⋆ ◎ ((id⟷ ⊗ swap₊) ◎ (id⟷ ◎ unite⋆))
          ⇔⟨ resp◎⇔ id⇔ (resp◎⇔ id⇔ idl◎l) ⟩
        uniti⋆ ◎ ((id⟷ ⊗ swap₊) ◎ unite⋆)
          ⇔⟨ assoc◎l ⟩
        (uniti⋆ ◎ (id⟷ ⊗ swap₊)) ◎ unite⋆
          ⇔⟨ resp◎⇔ unitil⋆⇔ id⇔ ⟩
        (swap₊ ◎ uniti⋆) ◎ unite⋆
          ⇔⟨ assoc◎r ⟩
        swap₊ ◎ (uniti⋆ ◎ unite⋆)
          ⇔⟨ resp◎⇔ id⇔ linv◎l ⟩
        swap₊ ◎ id⟷
          ⇔⟨ idr◎l ⟩
        swap₊ ▤

-- The equivalence ⇔ of paths is rich enough to make U a 1groupoid:
-- the points are types (t : U); the 1paths are ⟷; and the 2paths
-- between them are based on the simplification rules ⇔ 

G' : 1Groupoid
G' = record
        { set = U
        ; _↝_ = _⟷_
        ; _≈_ = _⇔_
        ; id  = id⟷
        ; _∘_ = λ p q → q ◎ p
        ; _⁻¹ = !
        ; lneutr = λ _ → idr◎l
        ; rneutr = λ _ → idl◎l
        ; assoc  = λ _ _ _ → assoc◎l
        ; equiv = record { 
            refl  = id⇔
          ; sym   = 2!
          ; trans = trans⇔
          }
        ; linv = λ {t₁} {t₂} α → linv◎l
        ; rinv = λ {t₁} {t₂} α → rinv◎l
        ; ∘-resp-≈ = λ p∼q r∼s → resp◎⇔ r∼s p∼q 
        }

------------------------------------------------------------------------------
-- The syntactic combinators are rich enough to define the groupoid structure. Now
-- we investigate whether they are complete.

-- Inverting permutations to a canonical syntactic combinator

perm2c : {t₁ t₂ : U} → (size t₁ ≡ size t₂) → Permutation (size t₁) → (t₁ ⟷ t₂)
perm2c {ZERO} {ZERO} refl ([] , f) = id⟷
perm2c {ZERO} {ONE} () (cauchy , f)
perm2c {ZERO} {PLUS t₂ t₃} sp ([] , f) = {!!} 
perm2c {ZERO} {TIMES t₂ t₃} sp ([] , f) = {!!}
perm2c {ZERO} {BOOL} () (cauchy , f)
perm2c {ONE} {ZERO} () (cauchy , f)
perm2c {ONE} {ONE} refl (zero ∷ [] , f) = id⟷
perm2c {ONE} {ONE} refl (suc () ∷ [] , f)
perm2c {ONE} {PLUS t₂ t₃} sp (cauchy , f) = {!!}
perm2c {ONE} {TIMES t₂ t₃} sp (cauchy , f) = {!!}
perm2c {ONE} {BOOL} () (cauchy , f)
perm2c {PLUS t₁ t₂} {ZERO} sp (cauchy , f) = {!!}
perm2c {PLUS t₁ t₂} {ONE} sp (cauchy , f) = {!!}
perm2c {PLUS t₁ t₂} {PLUS t₃ t₄} sp (cauchy , f) = {!!}
perm2c {PLUS t₁ t₂} {TIMES t₃ t₄} sp (cauchy , f) = {!!}
perm2c {PLUS t₁ t₂} {BOOL} sp (cauchy , f) = {!!}
perm2c {TIMES t₁ t₂} {ZERO} sp (cauchy , f) = {!!}
perm2c {TIMES t₁ t₂} {ONE} sp (cauchy , f) = {!!}
perm2c {TIMES t₁ t₂} {PLUS t₃ t₄} sp (cauchy , f) = {!!}
perm2c {TIMES t₁ t₂} {TIMES t₃ t₄} sp (cauchy , f) = {!!}
perm2c {TIMES t₁ t₂} {BOOL} sp (cauchy , f) = {!!}
perm2c {BOOL} {ZERO} () (cauchy , f)
perm2c {BOOL} {ONE} () (cauchy , f)
perm2c {BOOL} {PLUS t₂ t₃} sp (cauchy , f) = {!!}
perm2c {BOOL} {TIMES t₂ t₃} sp (cauchy , f) = {!!}
perm2c {BOOL} {BOOL} refl (zero ∷ zero ∷ [] , f) with f {zero} {suc zero}
... | x = ⊥-elim ((m≢1+m+n) 0 (cong toℕ (x refl))) 
perm2c {BOOL} {BOOL} refl (zero ∷ suc zero ∷ [] , f) = id⟷
perm2c {BOOL} {BOOL} refl (zero ∷ suc (suc ()) ∷ [] , f)
perm2c {BOOL} {BOOL} refl (suc zero ∷ zero ∷ [] , f) = NOT
perm2c {BOOL} {BOOL} refl (suc (suc ()) ∷ zero ∷ [] , f)
perm2c {BOOL} {BOOL} refl (suc zero ∷ suc zero ∷ [] , f) with f {zero} {suc zero}
... | x = ⊥-elim ((m≢1+m+n) 0 (cong toℕ (x refl))) 
perm2c {BOOL} {BOOL} refl (suc zero ∷ suc (suc ()) ∷ [] , f)
perm2c {BOOL} {BOOL} refl (suc (suc ()) ∷ suc zero ∷ [] , f)
perm2c {BOOL} {BOOL} refl (suc (suc ()) ∷ suc (suc b) ∷ [] , f) 

------------------------------------------------------------------------------
-- Soundness and completeness
-- 
-- Proof of soundness and completeness: now we want to verify that ⇔
-- is sound and complete with respect to ∼. The statement to prove is
-- that for all c₁ and c₂, we have c₁ ∼ c₂ iff c₁ ⇔ c₂

soundness : {t₁ t₂ : U} {c₁ c₂ : t₁ ⟷ t₂} → (c₁ ⇔ c₂) → (c₁ ∼ c₂)
soundness α = {!!} 

-- The idea is to invert evaluation and use that to extract from each
-- extensional representation of a combinator, a canonical syntactic
-- representative

canonical : {t₁ t₂ : U} → (t₁ ⟷ t₂) → (t₁ ⟷ t₂)
canonical c = perm2c (size≡ c) (c2perm c)

-- Note that if c₁ ⇔ c₂, then by soundness c₁ ∼ c₂ and hence their
-- canonical representatives are identical. 

-- If we try to show we defined cauchy and perm in a compatible way,
-- this fails (under --without-K) basically what we get is (which
-- would complete the proof), but in some case the middle proof is
-- assuredly 'refl', which cannot be eliminated.
-- cauchy⇒perm : {t₁ t₂ : U} → (c₁ c₂ : t₁ ⟷ t₂) →
--   c2cauchy c₁ ≡ c2cauchy c₂ → c2perm c₁ ≡ c2perm c₂

canonicalWellDefined : {t₁ t₂ : U} {c₁ c₂ : t₁ ⟷ t₂} → 
  (c₁ ⇔ c₂) → (canonical c₁ ≡ canonical c₂)
canonicalWellDefined {t₁} {t₂} {c₁} {c₂} α =
  cong₂ perm2c (size∼ c₁ c₂) {!soundness α!} 
-- cong₂ perm2c (size∼ c₁ c₂) (cauchy⇒perm c₁ c₂ (soundness α))
--  cong₂ {!!} (size∼ c₁ c₂) (soundness α) 

-- If we can prove that every combinator is equal to its normal form
-- then we can prove completeness.

inversion : {t₁ t₂ : U} (c : t₁ ⟷ t₂) → c ⇔ canonical c
inversion (c₁ ◎ c₂) = {!!} 
inversion {PLUS ZERO t} {.t} unite₊ = {!!} 
inversion {t} {PLUS ZERO .t} uniti₊ = {!!} 
inversion {PLUS t₁ t₂} {PLUS .t₂ .t₁} swap₊ = {!!} 
inversion {PLUS t₁ (PLUS t₂ t₃)} {PLUS (PLUS .t₁ .t₂) .t₃} assocl₊ = {!!} 
inversion {PLUS (PLUS t₁ t₂) t₃} {PLUS .t₁ (PLUS .t₂ .t₃)} assocr₊ = {!!}
inversion {TIMES ONE t} {.t} unite⋆ = {!!}
inversion {t} {TIMES ONE .t} uniti⋆ = {!!} 
inversion {TIMES t₁ t₂} {TIMES .t₂ .t₁} swap⋆ = {!!} 
inversion {TIMES t₁ (TIMES t₂ t₃)} {TIMES (TIMES .t₁ .t₂) .t₃} assocl⋆ = {!!}
inversion {TIMES (TIMES t₁ t₂) t₃} {TIMES .t₁ (TIMES .t₂ .t₃)} assocr⋆ = {!!}
inversion {TIMES .ZERO t} {ZERO} distz = {!!} 
inversion {ZERO} {TIMES ZERO t} factorz = {!!} 
inversion {TIMES (PLUS t₁ t₂) t₃} {PLUS (TIMES .t₁ .t₃) (TIMES .t₂ .t₃)} dist = {!!}
inversion {PLUS (TIMES t₁ t₃) (TIMES t₂ .t₃)} {TIMES (PLUS .t₁ .t₂) .t₃} factor = {!!}
inversion {t} {.t} id⟷ = {!!} 
inversion {PLUS t₁ t₂} {PLUS t₃ t₄} (c₁ ⊕ c₂) = {!!} 
inversion {TIMES t₁ t₂} {TIMES t₃ t₄} (c₁ ⊗ c₂) = {!!} 
inversion {PLUS ONE ONE} {BOOL} foldBool = {!!} 
inversion {BOOL} {PLUS ONE ONE} unfoldBool = {!!} 

resp≡⇔ : {t₁ t₂ : U} {c₁ c₂ : t₁ ⟷ t₂} → (c₁ ≡ c₂) → (c₁ ⇔ c₂)
resp≡⇔ {t₁} {t₂} {c₁} {c₂} p rewrite p = id⇔ 

completeness : {t₁ t₂ : U} {c₁ c₂ : t₁ ⟷ t₂} → (c₁ ∼ c₂) → (c₁ ⇔ c₂)
completeness {t₁} {t₂} {c₁} {c₂} c₁∼c₂ = 
  c₁
    ⇔⟨ inversion c₁ ⟩
  canonical c₁
    ⇔⟨  {!!} ⟩ 
--    ⇔⟨  resp≡⇔ (cong₂ {!!} (size∼ c₁ c₂) c₁∼c₂) ⟩ 
  canonical c₂
    ⇔⟨ 2! (inversion c₂) ⟩ 
  c₂ ▤

------------------------------------------------------------------------------


